thys/Superposition_Calculus/Superposition.thy
@@ -117,8 +117,8 @@ where
     welltyped_imgu_on (clause.vars (E \<cdot> \<rho>\<^sub>1) \<union> clause.vars (D \<cdot> \<rho>\<^sub>2)) \<V>\<^sub>3 (t\<^sub>1 \<cdot>t \<rho>\<^sub>1) (t\<^sub>2 \<cdot>t \<rho>\<^sub>2) \<mu> \<Longrightarrow>
     \<forall>x \<in> clause.vars E. \<V>\<^sub>1 x = \<V>\<^sub>3 (term.rename \<rho>\<^sub>1 x) \<Longrightarrow>
     \<forall>x \<in> clause.vars D. \<V>\<^sub>2 x = \<V>\<^sub>3 (term.rename \<rho>\<^sub>2 x) \<Longrightarrow>
-    is_welltyped_on (clause.vars E) \<V>\<^sub>1 \<rho>\<^sub>1 \<Longrightarrow>
-    is_welltyped_on (clause.vars D) \<V>\<^sub>2 \<rho>\<^sub>2 \<Longrightarrow>
+    term.subst.is_welltyped_on (clause.vars E) \<V>\<^sub>1 \<rho>\<^sub>1 \<Longrightarrow>
+    term.subst.is_welltyped_on (clause.vars D) \<V>\<^sub>2 \<rho>\<^sub>2 \<Longrightarrow>
     (\<And>\<tau> \<tau>'. typed \<V>\<^sub>2 t\<^sub>2 \<tau> \<Longrightarrow> typed \<V>\<^sub>2 t\<^sub>2' \<tau>' \<Longrightarrow> \<tau> = \<tau>') \<Longrightarrow>
     \<not> (E \<cdot> \<rho>\<^sub>1 \<odot> \<mu> \<preceq>\<^sub>c D \<cdot> \<rho>\<^sub>2 \<odot> \<mu>) \<Longrightarrow>
     (\<P> = Pos 
@@ -168,8 +168,8 @@ where
     welltyped_imgu_on (clause.vars (E \<cdot> \<rho>\<^sub>1) \<union> clause.vars (D \<cdot> \<rho>\<^sub>2)) \<V>\<^sub>3 (t\<^sub>1 \<cdot>t \<rho>\<^sub>1) (t\<^sub>2 \<cdot>t \<rho>\<^sub>2) \<mu> \<Longrightarrow>
     \<forall>x \<in> clause.vars E. \<V>\<^sub>1 x = \<V>\<^sub>3 (term.rename \<rho>\<^sub>1 x) \<Longrightarrow>
     \<forall>x \<in> clause.vars D. \<V>\<^sub>2 x = \<V>\<^sub>3 (term.rename \<rho>\<^sub>2 x) \<Longrightarrow>
-    is_welltyped_on (clause.vars E) \<V>\<^sub>1 \<rho>\<^sub>1 \<Longrightarrow>
-    is_welltyped_on (clause.vars D) \<V>\<^sub>2 \<rho>\<^sub>2 \<Longrightarrow>
+    term.subst.is_welltyped_on (clause.vars E) \<V>\<^sub>1 \<rho>\<^sub>1 \<Longrightarrow>
+    term.subst.is_welltyped_on (clause.vars D) \<V>\<^sub>2 \<rho>\<^sub>2 \<Longrightarrow>
     (\<And>\<tau> \<tau>'. typed \<V>\<^sub>2 t\<^sub>2 \<tau> \<Longrightarrow> typed \<V>\<^sub>2 t\<^sub>2' \<tau>' \<Longrightarrow> \<tau> = \<tau>') \<Longrightarrow>
     \<not> (E \<cdot> \<rho>\<^sub>1 \<odot> \<mu> \<preceq>\<^sub>c D \<cdot> \<rho>\<^sub>2 \<odot> \<mu>) \<Longrightarrow>
     select E = {#} \<Longrightarrow>
@@ -211,8 +211,8 @@ where
     welltyped_imgu_on (clause.vars (E \<cdot> \<rho>\<^sub>1) \<union> clause.vars (D \<cdot> \<rho>\<^sub>2)) \<V>\<^sub>3 (t\<^sub>1 \<cdot>t \<rho>\<^sub>1) (t\<^sub>2 \<cdot>t \<rho>\<^sub>2) \<mu> \<Longrightarrow>
     \<forall>x \<in> clause.vars E. \<V>\<^sub>1 x = \<V>\<^sub>3 (term.rename \<rho>\<^sub>1 x) \<Longrightarrow>
     \<forall>x \<in> clause.vars D. \<V>\<^sub>2 x = \<V>\<^sub>3 (term.rename \<rho>\<^sub>2 x) \<Longrightarrow>
-    is_welltyped_on (clause.vars E) \<V>\<^sub>1 \<rho>\<^sub>1 \<Longrightarrow>
-    is_welltyped_on (clause.vars D) \<V>\<^sub>2 \<rho>\<^sub>2 \<Longrightarrow>
+    term.subst.is_welltyped_on (clause.vars E) \<V>\<^sub>1 \<rho>\<^sub>1 \<Longrightarrow>
+    term.subst.is_welltyped_on (clause.vars D) \<V>\<^sub>2 \<rho>\<^sub>2 \<Longrightarrow>
     (\<And>\<tau> \<tau>'. typed \<V>\<^sub>2 t\<^sub>2 \<tau> \<Longrightarrow> typed \<V>\<^sub>2 t\<^sub>2' \<tau>' \<Longrightarrow> \<tau> = \<tau>') \<Longrightarrow>
     \<not> (E \<cdot> \<rho>\<^sub>1 \<odot> \<mu> \<preceq>\<^sub>c D \<cdot> \<rho>\<^sub>2 \<odot> \<mu>) \<Longrightarrow>
     select E = {#} \<and> 
