thys/Superposition_Calculus/Superposition_Completeness.thy
@@ -27,7 +27,7 @@ lemma eq_resolution_lifting:
     C_grounding: "clause.is_ground (C \<cdot> \<gamma>)" and
     select: "clause.from_ground (select\<^sub>G D\<^sub>G) = (select D) \<cdot> \<gamma>" and
     D_is_welltyped: "clause.is_welltyped \<V> D" and
-    \<gamma>_is_welltyped: "is_welltyped_on (clause.vars D) \<V> \<gamma>" and
+    \<gamma>_is_welltyped: "term.subst.is_welltyped_on (clause.vars D) \<V> \<gamma>" and
     \<V>: "infinite_variables_per_type \<V>"
   obtains C'
   where
@@ -230,7 +230,7 @@ proof(cases D\<^sub>G C\<^sub>G rule: ground.eq_resolution.cases)
           unfolding D l
           by auto
 
-        then show "is_welltyped_on (clause.vars (C' \<cdot> \<mu>)) \<V> \<gamma>"
+        then show "term.subst.is_welltyped_on (clause.vars (C' \<cdot> \<mu>)) \<V> \<gamma>"
           using D_is_welltyped \<gamma>_is_welltyped
           by blast
       next
@@ -261,7 +261,7 @@ lemma eq_factoring_lifting:
     C_grounding: "clause.is_ground (C \<cdot> \<gamma>)" and
     select: "clause.from_ground (select\<^sub>G D\<^sub>G) = (select D) \<cdot> \<gamma>" and
     D_is_welltyped: "clause.is_welltyped \<V> D" and
-    \<gamma>_is_welltyped: "is_welltyped_on (clause.vars D) \<V> \<gamma>" and
+    \<gamma>_is_welltyped: "term.subst.is_welltyped_on (clause.vars D) \<V> \<gamma>" and
     \<V>: "infinite_variables_per_type \<V>"
   obtains C' 
   where
@@ -446,7 +446,7 @@ proof(cases D\<^sub>G C\<^sub>G rule: ground.eq_factoring.cases)
           unfolding D l\<^sub>1 l\<^sub>2
           by auto
 
-        then show "is_welltyped_on (clause.vars ?C') \<V> \<gamma>"
+        then show "term.subst.is_welltyped_on (clause.vars ?C') \<V> \<gamma>"
           using D_is_welltyped \<gamma>_is_welltyped
           by blast
       next
@@ -487,10 +487,10 @@ lemma superposition_lifting:
     select_from_D: "clause.from_ground (select\<^sub>G D\<^sub>G) = (select D) \<cdot> \<rho>\<^sub>2 \<odot> \<gamma>" and
     E_is_welltyped: "clause.is_welltyped \<V>\<^sub>1 E" and
     D_is_welltyped: "clause.is_welltyped \<V>\<^sub>2 D" and
-    \<rho>\<^sub>1_\<gamma>_is_welltyped: "is_welltyped_on (clause.vars E) \<V>\<^sub>1 (\<rho>\<^sub>1 \<odot> \<gamma>)" and
-    \<rho>\<^sub>2_\<gamma>_is_welltyped: "is_welltyped_on (clause.vars D) \<V>\<^sub>2 (\<rho>\<^sub>2 \<odot> \<gamma>)" and
-    \<rho>\<^sub>1_is_welltyped: "is_welltyped_on (clause.vars E) \<V>\<^sub>1 \<rho>\<^sub>1" and
-    \<rho>\<^sub>2_is_welltyped: "is_welltyped_on (clause.vars D) \<V>\<^sub>2 \<rho>\<^sub>2" and
+    \<rho>\<^sub>1_\<gamma>_is_welltyped: "term.subst.is_welltyped_on (clause.vars E) \<V>\<^sub>1 (\<rho>\<^sub>1 \<odot> \<gamma>)" and
+    \<rho>\<^sub>2_\<gamma>_is_welltyped: "term.subst.is_welltyped_on (clause.vars D) \<V>\<^sub>2 (\<rho>\<^sub>2 \<odot> \<gamma>)" and
+    \<rho>\<^sub>1_is_welltyped: "term.subst.is_welltyped_on (clause.vars E) \<V>\<^sub>1 \<rho>\<^sub>1" and
+    \<rho>\<^sub>2_is_welltyped: "term.subst.is_welltyped_on (clause.vars D) \<V>\<^sub>2 \<rho>\<^sub>2" and
     \<V>\<^sub>1: "infinite_variables_per_type \<V>\<^sub>1" and
     \<V>\<^sub>2: "infinite_variables_per_type \<V>\<^sub>2" and
     not_redundant: "\<iota>\<^sub>G \<notin> ground.Red_I N\<^sub>G"
@@ -790,7 +790,7 @@ proof(cases D\<^sub>G E\<^sub>G C\<^sub>G rule: ground.superposition.cases)
               using E_grounding
               by simp
 
-            show "is_welltyped_on (clause.vars E) \<V>\<^sub>1 (\<rho>\<^sub>1 \<odot> \<gamma>')"
+            show "term.subst.is_welltyped_on (clause.vars E) \<V>\<^sub>1 (\<rho>\<^sub>1 \<odot> \<gamma>')"
             proof(intro is_welltyped_on_subst_compose \<rho>\<^sub>1_is_welltyped)
               
               have "welltyped \<V>\<^sub>1 ?t\<^sub>G (\<V>\<^sub>1 x)"
@@ -841,7 +841,7 @@ proof(cases D\<^sub>G E\<^sub>G C\<^sub>G rule: ground.superposition.cases)
                     by auto
 
                   then show ?thesis
-                    using that welltyped.explicit_replace_\<V>_iff[of _ \<V>\<^sub>2 \<V>\<^sub>1]
+                    using that term.welltyped.explicit_replace_\<V>_iff[of _ \<V>\<^sub>2 \<V>\<^sub>1]
                     by simp
                 qed
 
@@ -849,11 +849,12 @@ proof(cases D\<^sub>G E\<^sub>G C\<^sub>G rule: ground.superposition.cases)
                   by auto              
               qed
 
-              moreover have "is_welltyped_on (\<Union> (term.vars ` \<rho>\<^sub>1 ` clause.vars E)) \<V>\<^sub>1 \<gamma>"
+              moreover have "term.subst.is_welltyped_on (\<Union> (term.vars ` \<rho>\<^sub>1 ` clause.vars E)) \<V>\<^sub>1 \<gamma>"
                 by (intro is_welltyped_on_subst_compose_renaming \<rho>\<^sub>1_\<gamma>_is_welltyped
                     \<rho>\<^sub>1_is_welltyped \<rho>\<^sub>1)
 
-              ultimately show "is_welltyped_on (\<Union> (term.vars ` \<rho>\<^sub>1 ` clause.vars E)) \<V>\<^sub>1 \<gamma>'"
+              ultimately show 
+                "term.subst.is_welltyped_on (\<Union> (term.vars ` \<rho>\<^sub>1 ` clause.vars E)) \<V>\<^sub>1 \<gamma>'"
                 unfolding \<gamma>'_def
                 by simp
             qed
@@ -1038,14 +1039,15 @@ proof(cases D\<^sub>G E\<^sub>G C\<^sub>G rule: ground.superposition.cases)
     \<V>\<^sub>3: "infinite_variables_per_type \<V>\<^sub>3"
     using clause.obtain_merged_\<V>[OF \<rho>\<^sub>1 \<rho>\<^sub>2 rename_apart \<V>\<^sub>1 \<V>\<^sub>2 clause.finite_vars].
 
-  have \<gamma>_is_welltyped: "is_welltyped_on (clause.vars (E \<cdot> \<rho>\<^sub>1) \<union> clause.vars (D \<cdot> \<rho>\<^sub>2)) \<V>\<^sub>3 \<gamma>"
+  have \<gamma>_is_welltyped: 
+    "term.subst.is_welltyped_on (clause.vars (E \<cdot> \<rho>\<^sub>1) \<union> clause.vars (D \<cdot> \<rho>\<^sub>2)) \<V>\<^sub>3 \<gamma>"
   proof(unfold Set.ball_Un, intro conjI)
 
-    show "is_welltyped_on (clause.vars (E \<cdot> \<rho>\<^sub>1)) \<V>\<^sub>3 \<gamma>"
+    show "term.subst.is_welltyped_on (clause.vars (E \<cdot> \<rho>\<^sub>1)) \<V>\<^sub>3 \<gamma>"
       using clause.is_welltyped.renaming_grounding[OF \<rho>\<^sub>1 \<rho>\<^sub>1_\<gamma>_is_welltyped E_grounding \<V>\<^sub>1_\<V>\<^sub>3].
   next
  
-    show "is_welltyped_on (clause.vars (D \<cdot> \<rho>\<^sub>2)) \<V>\<^sub>3 \<gamma>"
+    show "term.subst.is_welltyped_on (clause.vars (D \<cdot> \<rho>\<^sub>2)) \<V>\<^sub>3 \<gamma>"
       using clause.is_welltyped.renaming_grounding[OF \<rho>\<^sub>2 \<rho>\<^sub>2_\<gamma>_is_welltyped D_grounding \<V>\<^sub>2_\<V>\<^sub>3].
   qed
 
@@ -1070,8 +1072,8 @@ proof(cases D\<^sub>G E\<^sub>G C\<^sub>G rule: ground.superposition.cases)
         by auto
 
       then have "welltyped \<V>\<^sub>3 (term.from_ground t\<^sub>G\<^sub>1) \<tau>" 
-        using welltyped.is_ground_typed
-        by (meson term.ground_is_ground welltyped.explicit_is_ground_typed)
+        using term.welltyped.is_ground_typed
+        by (meson term.ground_is_ground term.welltyped.explicit_is_ground_typed)
 
       then have "welltyped \<V>\<^sub>3 (t\<^sub>1 \<cdot>t \<rho>\<^sub>1 \<odot> \<gamma>) \<tau>" "welltyped \<V>\<^sub>3 (t\<^sub>2 \<cdot>t \<rho>\<^sub>2 \<odot> \<gamma>) \<tau>"
         using t\<^sub>1_\<gamma> t\<^sub>2_\<gamma>
@@ -1105,7 +1107,7 @@ proof(cases D\<^sub>G E\<^sub>G C\<^sub>G rule: ground.superposition.cases)
 
     show superposition: "superposition (D, \<V>\<^sub>2) (E, \<V>\<^sub>1) (C', \<V>\<^sub>3)"
     proof(rule superpositionI; 
-           ((rule \<rho>\<^sub>1 \<rho>\<^sub>2 E D l\<^sub>1 l\<^sub>2 t\<^sub>1_is_Fun imgu rename_apart \<rho>\<^sub>1_is_welltyped \<rho>\<^sub>2_is_welltyped \<V>\<^sub>1 \<V>\<^sub>2 C' 
+           ((rule \<rho>\<^sub>1 \<rho>\<^sub>2 E D l\<^sub>1 l\<^sub>2 t\<^sub>1_is_Fun imgu rename_apart \<rho>\<^sub>1_is_welltyped \<rho>\<^sub>2_is_welltyped \<V>\<^sub>1 \<V>\<^sub>2 C'
                \<V>\<^sub>1_\<V>\<^sub>3 \<V>\<^sub>2_\<V>\<^sub>3)+)?)
 
       show "?\<P> \<in> {Pos, Neg}"
@@ -1336,8 +1338,8 @@ proof(cases D\<^sub>G E\<^sub>G C\<^sub>G rule: ground.superposition.cases)
           by simp
       next
 
-        show "is_welltyped_on (clause.vars C') \<V>\<^sub>3 \<gamma>"
-        proof(rule is_welltyped_on_subset[OF \<gamma>_is_welltyped])
+        show "term.subst.is_welltyped_on (clause.vars C') \<V>\<^sub>3 \<gamma>"
+        proof(rule term.is_welltyped_on_subset[OF \<gamma>_is_welltyped])
 
           show "clause.vars C' \<subseteq> clause.vars (E \<cdot> \<rho>\<^sub>1) \<union> clause.vars (D \<cdot> \<rho>\<^sub>2)"
           proof (unfold subset_eq, intro ballI)
@@ -1429,7 +1431,7 @@ lemma single_premise_ground_instance:
     clause.is_ground (D \<cdot> \<gamma>); 
     clause.is_ground (C \<cdot> \<gamma>);
     clause.from_ground (select\<^sub>G (clause.to_ground (D \<cdot> \<gamma>))) = select D \<cdot> \<gamma>; 
-    clause.is_welltyped \<V> D; is_welltyped_on (clause.vars D) \<V> \<gamma>;
+    clause.is_welltyped \<V> D; term.subst.is_welltyped_on (clause.vars D) \<V> \<gamma>;
     infinite_variables_per_type \<V>;
     \<And>C'. \<lbrakk>
         inference (D, \<V>) (C', \<V>);
@@ -1456,7 +1458,7 @@ proof-
   obtain D \<gamma> \<V> where
     D_grounding: "clause.is_ground (D \<cdot> \<gamma>)" and
     D_is_welltyped: "clause.is_welltyped \<V> D" and
-    \<gamma>_is_welltyped: "is_welltyped_on (clause.vars D) \<V> \<gamma>" and
+    \<gamma>_is_welltyped: "term.subst.is_welltyped_on (clause.vars D) \<V> \<gamma>" and
     \<V>: "infinite_variables_per_type \<V>" and
     D_in_N: "(D, \<V>)\<in>N" and 
     "select\<^sub>G D\<^sub>G = clause.to_ground (select D \<cdot> \<gamma>)"
@@ -1542,7 +1544,7 @@ proof-
   obtain E \<V>\<^sub>1 \<gamma>\<^sub>1 where
     E_grounding: "clause.is_ground (E \<cdot> \<gamma>\<^sub>1)" and
     E_is_welltyped: "clause.is_welltyped \<V>\<^sub>1 E" and
-    \<gamma>\<^sub>1_is_welltyped: "is_welltyped_on (clause.vars E) \<V>\<^sub>1 \<gamma>\<^sub>1" and
+    \<gamma>\<^sub>1_is_welltyped: "term.subst.is_welltyped_on (clause.vars E) \<V>\<^sub>1 \<gamma>\<^sub>1" and
     \<V>\<^sub>1: "infinite_variables_per_type \<V>\<^sub>1" and
     E_in_N: "(E, \<V>\<^sub>1)\<in>N" and 
     "select\<^sub>G E\<^sub>G = clause.to_ground (select E \<cdot> \<gamma>\<^sub>1)"
@@ -1558,7 +1560,7 @@ proof-
   obtain D \<V>\<^sub>2 \<gamma>\<^sub>2 where
     D_grounding: "clause.is_ground (D \<cdot> \<gamma>\<^sub>2)" and
     D_is_welltyped: "clause.is_welltyped \<V>\<^sub>2 D" and
-    \<gamma>\<^sub>2_is_welltyped: "is_welltyped_on (clause.vars D) \<V>\<^sub>2 \<gamma>\<^sub>2" and
+    \<gamma>\<^sub>2_is_welltyped: "term.subst.is_welltyped_on (clause.vars D) \<V>\<^sub>2 \<gamma>\<^sub>2" and
     \<V>\<^sub>2: "infinite_variables_per_type \<V>\<^sub>2" and
     D_in_N: "(D, \<V>\<^sub>2)\<in>N" and 
     "select\<^sub>G D\<^sub>G = clause.to_ground (select D \<cdot> \<gamma>\<^sub>2)"
@@ -1575,8 +1577,8 @@ proof-
     \<rho>\<^sub>1: "term_subst.is_renaming \<rho>\<^sub>1" and
     \<rho>\<^sub>2: "term_subst.is_renaming \<rho>\<^sub>2" and
     rename_apart:  "clause.vars (E \<cdot> \<rho>\<^sub>1) \<inter> clause.vars (D \<cdot> \<rho>\<^sub>2) = {}" and
-    \<rho>\<^sub>1_is_welltyped: "is_welltyped_on (clause.vars E) \<V>\<^sub>1 \<rho>\<^sub>1" and
-    \<rho>\<^sub>2_is_welltyped: "is_welltyped_on (clause.vars D) \<V>\<^sub>2 \<rho>\<^sub>2" and
+    \<rho>\<^sub>1_is_welltyped: "term.subst.is_welltyped_on (clause.vars E) \<V>\<^sub>1 \<rho>\<^sub>1" and
+    \<rho>\<^sub>2_is_welltyped: "term.subst.is_welltyped_on (clause.vars D) \<V>\<^sub>2 \<rho>\<^sub>2" and
     \<gamma>\<^sub>1_\<gamma>: "\<forall>X \<subseteq> clause.vars E. \<forall>x\<in> X. \<gamma>\<^sub>1 x = (\<rho>\<^sub>1 \<odot> \<gamma>) x" and
     \<gamma>\<^sub>2_\<gamma>: "\<forall>X \<subseteq> clause.vars D. \<forall>x\<in> X. \<gamma>\<^sub>2 x = (\<rho>\<^sub>2 \<odot> \<gamma>) x"
     using 
@@ -1599,11 +1601,11 @@ proof-
     using clause.subst_eq \<gamma>\<^sub>2_\<gamma> D\<^sub>G
     by fastforce
 
-  have \<rho>\<^sub>1_\<gamma>_is_welltyped: "is_welltyped_on (clause.vars E) \<V>\<^sub>1 (\<rho>\<^sub>1 \<odot> \<gamma>)"
+  have \<rho>\<^sub>1_\<gamma>_is_welltyped: "term.subst.is_welltyped_on (clause.vars E) \<V>\<^sub>1 (\<rho>\<^sub>1 \<odot> \<gamma>)"
     using \<gamma>\<^sub>1_is_welltyped \<gamma>\<^sub>1_\<gamma>
     by fastforce
 
-  have \<rho>\<^sub>2_\<gamma>_is_welltyped: "is_welltyped_on (clause.vars D) \<V>\<^sub>2 (\<rho>\<^sub>2 \<odot> \<gamma>)"
+  have \<rho>\<^sub>2_\<gamma>_is_welltyped: "term.subst.is_welltyped_on (clause.vars D) \<V>\<^sub>2 (\<rho>\<^sub>2 \<odot> \<gamma>)"
     using \<gamma>\<^sub>2_is_welltyped \<gamma>\<^sub>2_\<gamma>
     by fastforce
 
